Moved binary tree search as exercise23 in chapter01 Modifications to exercises 21 and 22 in chapter01

chapter01/solutions/exercise22_solution.dfy
@@ -1,19 +1,29 @@
 datatype Tree = Nil | Node(value:int, left:Tree, right:Tree)
 
-function method I(t:Tree) : seq<int>
+function method TreeAsSequence(t:Tree) : seq<int>
 {
     if t.Nil? then []
-    else I(t.left) + [t.value] + I(t.right)
+    else TreeAsSequence(t.left) + [t.value] + TreeAsSequence(t.right)
 }
 
 predicate IsSortedTree(t:Tree) {
     if (t.Nil?) 
     then true 
     else
-        && (forall j | 0 <= j < |I(t.left)| :: I(t.left)[j] <= t.value)
-        && (forall j | 0 <= j < |I(t.right)| :: t.value <= I(t.right)[j])
+        && (forall j | 0 <= j < |TreeAsSequence(t.left)| :: TreeAsSequence(t.left)[j] <= t.value)
+        && (forall j | 0 <= j < |TreeAsSequence(t.right)| :: t.value <= TreeAsSequence(t.right)[j])
         && IsSortedTree(t.left)
         && IsSortedTree(t.right)
+}
+
+predicate SequenceIsSorted(s:seq<int>) {
+    forall i:nat,j:nat | i<j<|s| :: s[i] <= s[j]
+}
+
+lemma SortedTreeMeansSortedSequence(t:Tree)
+    requires IsSortedTree(t) 
+    ensures SequenceIsSorted(TreeAsSequence(t))
+{
 }
 
 method CheckIfSortedTree(t:Tree) returns (sorted:bool)
@@ -28,8 +38,8 @@ method CheckIfSortedTree(t:Tree) returns (sorted:bool)
             assert !IsSortedTree(t);
             return false;
         } else {
-            var leftSeq := I(t.left);
-            var rightSeq := I(t.right);
+            var leftSeq := TreeAsSequence(t.left);
+            var rightSeq := TreeAsSequence(t.right);
             var isValueAfterLeft:bool := |leftSeq| == 0 || leftSeq[|leftSeq|-1] <= t.value;
             var isValueBeforeRight:bool := |rightSeq| == 0 || t.value <= rightSeq[0];
             if(!isValueAfterLeft) {
@@ -37,17 +47,12 @@ method CheckIfSortedTree(t:Tree) returns (sorted:bool)
             } else if (!isValueBeforeRight) {
                 return false;
             } else {
-                ISorted(t.left);
-                ISorted(t.right);
+                SortedTreeMeansSortedSequence(t.left);
+                SortedTreeMeansSortedSequence(t.right);
                 return true;
             }
         }    
     }
 }
 
-lemma ISorted(t:Tree)
-    requires IsSortedTree(t) 
-    ensures forall j,k | 0 <= j <= k < |I(t)| :: I(t)[j] <= I(t)[k]
-{
-}
 
